started working on reshape

CCode/fact.c
@@ -1,7 +1,7 @@
 int factorial(int n) {
 	int acc = 1;
 
-	for (int i = 1; i <= n; ++i) {
+	for (int i = n; i > 0; --i) {
 		acc *= i;		
 	}
 
