Proofs/fact.v
@@ -1,9 +1,10 @@
 (* workaround for not having notation *)
+From iris.heap_lang Require proofmode notation.
 Module iris.
 
-From iris.heap_lang Require Import proofmode notation.
+Import proofmode notation.
 
-Definition factI : val :=
+Definition factI : heap_lang.expr :=
   rec: "factI" "n" :=
     if: "n" = #0 then #1 else "factI" * ("n" - #1)
     .
@@ -11,8 +12,96 @@ Definition factI : val :=
 End iris.
 
 Require Import Vloc.Lib.theory.
+Require Import Vloc.CCode.fact.
 
-(*Require Import Vloc.CCode.fact.*)
+Instance fact_ctx : refines_ctx := { gName := 1; nspace := nroot .@ "test"}.
+
+Instance CompSpecs : compspecs. make_compspecs prog. Defined.
+Definition Vprog : varspecs.  mk_varspecs prog. Defined.
+
+(* here, the refines we had before won't work... *)
+Definition int_relate vVST vHL :=
+  (!! (exists n : Z, vVST = Vint (Int.repr n) /\ vHL = LitV (heap_lang.LitInt n%Z)) && emp)%logic.
+
+Definition fspec :=
+  DECLARE _factorial
+  WITH gv: globals, ctx: ref_id, n : Z
+  PRE [ tint ]
+    PROP()
+    PARAMS(Vint (Int.repr n))
+    GLOBALS()
+    SEP(refines_right ctx (App iris.factI (Val (LitV (LitInt n)))))
+  POST [ tint ] 
+    EX v' : ival, EX v : val,
+    PROP()
+    RETURN(v)
+    SEP(refines_right ctx (ectxi_language.of_val v') * int_relate v v').
+
+Definition Gprog : funspecs := [fspec].
+
+Ltac print_goal := match goal with
+                   | |- ?p => idtac "GOAL IS: " p
+                   end.
+
+Lemma one_plus_zero : semax_body Vprog Gprog f_factorial fspec.
+Proof.
+  start_function. 
+  unfold iris.factI.
+  forward.
+
+  (*evar (thing : iexp).*)
+  (*assert ((PureExec True  1*)
+   (*(heap_lang.Rec "factI" "n"*)
+      (*(If (BinOp EqOp (Var "n") (Val (LitV (LitInt 0))))*)
+         (*(Val (LitV (LitInt 1)))*)
+         (*(BinOp MultOp (Var "factI")*)
+            (*(BinOp MinusOp (Var "n") (Val (LitV (LitInt 1))))))) thing)).*)
+            (*{*)
+              (*eapply (pure_recc _).*)
+            (*}*)
+
+  match goal with
+  | |- context[refines_right ctx ?expr] => 
+      reshape_expr expr ltac:(fun K e => 
+        replace expr with (fill K e) by (by rewrite ? fill_app);
+        evar (e' : iexp);
+        viewshift_SEP 0 (refines_right ctx (fill K e'));
+        first (
+          go_lower; 
+          eapply (refines_right_pure_r e e' _ _ _ K 1);
+          [try_pures | auto | auto]
+        );
+        simpl in e';
+        subst e'
+        )
+  end.
+  evar (e' : iexp);
+  match goal with
+  | |- context[refines_right ctx expr] =>
+      replace expr with () 
+  end.
 
 
 
+        go_lower; eapply (refines_right_pure_r _ _ _ _ _ K' 1) ) end.
+        [ try_pures | auto | auto ]; simpl in e''; subst e''
+     )
+  end.
+  eapply (refines_right_pure_r _ _ _ _ _ [] 1); [| auto | auto].
+  eapply (pure_exec_ctx (Λ := heap_lang) _ [Val (RecV "FactI" "n" _)]).
+
+  step_pure_r ctx.
+  unfold refines_right.
+  unfold spec_ctx.
+  unfold spec_inv.
+
+  evar (e' : iexp).
+  viewshift_SEP 0 (@refines_right theory.gName theory.nspace ctx e').
+  go_lower.
+  eapply (refines_right_pure_r _ _ _ _ _ [] 1); [| auto | auto].
+  eapply (pure_exec_ctx (Λ := heap_lang) _ [Val (RecV "FactI" "n" _)]).
+
+
+
+  forward_loop (acc).
+  
